src/cbor/pulse/raw/CBOR.Pulse.API.Det.C.fst
@@ -103,57 +103,11 @@ ensures
   res
 }
 
-fn cbor_det_mk_string_from_array (_: unit) : cbor_det_mk_string_from_array_t
-=
-  (ty: major_type_byte_string_or_text_string)
-  (a: A.array U8.t)
-  (len: U64.t)
-  (#p: perm)
-  (#v: Ghost.erased (Seq.seq U8.t))
-{
-  A.pts_to_len a;
-  let _ : squash (SZ.fits_u64) = assume SZ.fits_u64;
-  let s = S.from_array a (SZ.uint64_to_sizet len);
-  ghost fn aux (_: unit)
-    requires S.is_from_array a s ** pts_to s #p v
-    ensures A.pts_to a #p v
-  {
-    S.to_array s;
-  };
-  Trade.intro _ _ _ aux;
-  S.pts_to_len s;
-  let res = cbor_det_mk_string () ty s;
-  with p' v' . assert (cbor_det_match p' res (Spec.pack (Spec.CString ty v')));
-  Trade.trans (cbor_det_match p' res (Spec.pack (Spec.CString ty v'))) _ _;
-  res
-}
+let cbor_det_mk_string_from_array (_: unit) =
+  mk_string_from_array (cbor_det_mk_string ())
 
-fn cbor_det_mk_array_from_array (_: unit) : cbor_det_mk_array_from_array_t
-=
-  (a: A.array cbor_det_t)
-  (len: U64.t)
-  (#pa: perm)
-  (#va: Ghost.erased (Seq.seq cbor_det_t))
-  (#pv: perm)
-  (#vv: Ghost.erased (list Spec.cbor))
-{
-  A.pts_to_len a;
-  let _ : squash (SZ.fits_u64) = assume SZ.fits_u64;
-  let s = S.from_array a (SZ.uint64_to_sizet len);
-  ghost fn aux (_: unit)
-    requires S.is_from_array a s ** pts_to s #pa va
-    ensures A.pts_to a #pa va
-  {
-    S.to_array s;
-  };
-  Trade.intro _ _ _ aux;
-  Trade.reg_r (pts_to s #pa va) (A.pts_to a #pa va) (PM.seq_list_match va vv (cbor_det_match pv));
-  S.pts_to_len s;
-  let res = cbor_det_mk_array () s;
-  with p' v' . assert (cbor_det_match p' res (Spec.pack (Spec.CArray v')));
-  Trade.trans (cbor_det_match p' res (Spec.pack (Spec.CArray v'))) _ _;
-  res
-}
+let cbor_det_mk_array_from_array (_: unit) =
+  mk_array_from_array (cbor_det_mk_array ())
 
 let cbor_det_mk_map_from_array : mk_map_from_array_t cbor_det_match cbor_det_map_entry_match =
   mk_map_from_array (CBOR.Pulse.API.Base.mk_map_from_ref (CBOR.Pulse.API.Det.Type.dummy_cbor_det_t ()) (CBOR.Pulse.API.Det.Common.cbor_det_mk_map_gen ()))
